PREFIX bh: <https://linked.data.gov.au/def/wa-borehole/>
PREFIX dcterms: <http://purl.org/dc/terms/>
PREFIX owl: <http://www.w3.org/2002/07/owl#>
PREFIX prov: <http://www.w3.org/ns/prov#>
PREFIX rdfs: <http://www.w3.org/2000/01/rdf-schema#>
PREFIX sdo: <https://schema.org/>
PREFIX skos: <http://www.w3.org/2004/02/skos/core#>
PREFIX time: <http://www.w3.org/2006/time#>
PREFIX xsd: <http://www.w3.org/2001/XMLSchema#>

<https://linked.data.gov.au/def/wa-borehole>
    a owl:Ontology ;
    dcterms:provenance "Generated for the Geological Survey of WA in 2022, informed by Samples modelling undertaken for the Department of Agriculture, Water & the Environment's Biodiversity Data Repository, the Terrestrial Ecosystems Research Network's ontologies, Geoscience Australia samples modelling and the Geological Survey of Queensland's Boreholes work" ;
    owl:versionIRI bh:0.1 ;
    owl:versionInfo "0.2 draft"^^xsd:string ;
    skos:definition "The Geological Survey of Western Australia's profile of several Standards to characterise boreholes."@en ;
    skos:prefLabel "WA Borehole Profile" ;
    sdo:creator
        <https://orcid.org/0000-0001-5969-4893> ,
        <https://orcid.org/0000-0002-8742-7730> ;
    sdo:dateCreated "2022-06-29"^^xsd:date ;
    sdo:dateIssued "2000-01-01"^^xsd:date ;
    sdo:dateModified "2022-08-19"^^xsd:date ;
    sdo:publisher <https://linked.data.gov.au/org/gswa> ;
.

bh:GeologicalSiteType
    a owl:ObjectProperty ;
    skos:definition "The time period during which the borehole was drilled."@en ;
    skos:prefLabel "had drilling time"@en ;
    skos:usageNote "If the borehole was drilled at multiple times, add multiple :hasDrillingTime properties."@en ;
    sdo:domainIncludes bh:Borehole ;
.

bh:generated
    a owl:DatatypeProperty ;
    rdfs:domain bh:Relation ;
    rdfs:range xsd:boolean ;
    skos:definition "Specifies whether the relation was generated from document or extracted from the KB."@en ;
    skos:prefLabel "Generated"@en ;
.

bh:hadDrillingTime
    a owl:ObjectProperty ;
    rdfs:range time:ProperInterval ;
    skos:definition "The time period during which the borehole was drilled."@en ;
    skos:prefLabel "had drilling time"@en ;
    skos:usageNote "If the borehole was drilled at multiple times, add multiple :hasDrillingTime properties."@en ;
    sdo:domainIncludes bh:Borehole ;
.

bh:hasPurpose
    a owl:ObjectProperty ;
    rdfs:domain bh:Borehole ;
    rdfs:range skos:Concept ;
    owl:imports <https://linked.data.gov.au/def/borehole-purpose/> ;
    skos:definition "The reason for which this borehole was drilled."@en ;
    skos:prefLabel "Purpose" ;
    skos:usageNote "Purposes must be selected from the Borehole Purpose vocabulary. Multiple purposes may be selected. If purposes are time-bound, this should be indicated by assigning the purpose a time:hasTime property."@en ;
.

bh:operator
    a owl:ObjectProperty ;
    rdfs:subPropertyOf prov:wasAttributedTo ;
    skos:definition "An organisation that maintains/uses/runs the borehole."@en ;
    skos:prefLabel "operator"@en ;
    skos:usageNote "If the borehole was/is operated by multiple organisations, add multiple :operator properties. Different periods of operation, may have the specific operator indicated by qualifying the Entity (Borehole) / Agent (operator) relations, as per PROV-O's qualifiedAttribution pattern."@en ;
    sdo:domainIncludes bh:Borehole ;
.

<https://kurrawong.net>
    a sdo:Organization ;
    sdo:description "Kurrawong AI is a small, Artificial Intelligence, company in Australia specialising in Knowledge Graphs." ;
    sdo:identifier "31 353 542 036" ;
    sdo:name "Kurrawong AI" ;
    sdo:url "https://kurrawong.net"^^xsd:anyURI ;
.

<https://linked.data.gov.au/org/dmirs>
    a sdo:Organization ;
    sdo:identifier "69 410 335 356" ;
    sdo:name "Department of Mines, Industry Regulation & Safety" ;
    sdo:url "https://www.dmirs.wa.gov.au"^^xsd:anyURI ;
.

<https://linked.data.gov.au/org/gswa>
    a sdo:Organization ;
    sdo:name "Geological Survey of Western Australia" ;
    sdo:parentOrganization <https://linked.data.gov.au/org/dmirs> ;
    sdo:url "https://dmp.wa.gov.au/Geological-Survey/Geological-Survey-262.aspx"^^xsd:anyURI ;
.

bh:GeologicalSite
    a owl:Class ;
    rdfs:subClassOf bh:Thing ;
    skos:definition "The proximate geological features and locations that may be sampled or observed to determine the geological properties of an ultimate feature of interest."@en ;
    skos:prefLabel "Geological Site"@en ;
.

<https://orcid.org/0000-0001-5969-4893>
    sdo:email "david@crosslateral.com.au"^^xsd:anyURI ;
    sdo:name "David Crosswell" ;
.

<https://orcid.org/0000-0002-8742-7730>
    a sdo:Person ;
    sdo:affiliation <https://kurrawong.net> ;
    sdo:email "nick@kurrawong.net"^^xsd:anyURI ;
    sdo:name "Nicholas J. Car"@en ;
.

bh:Borehole
    a owl:Class ;
    rdfs:subClassOf bh:GeologicalSite ;
    skos:definition "A borehole is a narrow shaft bored in the ground. A borehole may be constructed for many different purposes, including the extraction of water, other liquids (such as petroleum) or gases (such as natural gas), as part of a geotechnical investigation, environmental site assessment, mineral exploration, temperature measurement, as a pilot hole for installing piers or underground utilities, for geothermal installations, or for underground storage of unwanted substances, e.g. in carbon capture and storage."@en ;
    skos:prefLabel "Borehole"@en ;
.

